haetae-topdown-easycrypt/post-freeze/VerifyUnpackV3PostDecodeThroughNttPostFreeze.ec
@@ -10,7 +10,9 @@ require import BArray2752 BArray8192 BArray32768 VerifyUnpackMode2Target
   VerifyUnpackV3AssemblyPostFreeze VerifyUnpackV3PreNttPostFreeze
   VerifyUnpackV3ExpandBoundsPostFreeze
   VerifyUnpackV3PreNttBoundPostFreeze
+  VerifyUnpackV3PreNttTightBoundPostFreeze
   VerifyUnpackV3NttBound17PostFreeze
+  VerifyUnpackV3NttTightBoundPostFreeze
   VerifyUnpackV3NttInstallPostFreeze
   VerifyUnpackV3MatrixProfilePostFreeze
   VerifyUnpackV3MatDoubleBoundsPostFreeze.
@@ -153,6 +155,83 @@ rewrite
 by auto.
 qed.
 
+lemma actual_verify_unpack_post_decode_pre_ntt_mode2_tight_bound
+    (bp0 : BArray8192.t) (vkp0 : BArray2752.t)
+    (mat0 : BArray32768.t) :
+  hoare [ActualVerifyUnpackPostDecodePreNttMode2.run :
+    bp = bp0 /\ vkp = vkp0 /\ matp = mat0 /\
+    VerifyUnpackVkM23CoefficientsPostFreeze.decoded_coeff_prefix
+      bp0 vkp0 mode2_vec_words /\
+    VerifyUnpackV3ExpandBoundsPostFreeze.expanded_mode2_prefix_bound mat0 /\
+    VerifyUnpackV3PreNttBoundPostFreeze.pre_ntt_source_bound vkp0 mat0
+    ==>
+    VerifyUnpackV3PreNttPostFreeze.pre_ntt_prefix
+      vkp0 res.`2 res.`1 mode2_vec_words /\
+    mat_firstcol_frame mat0 res.`2 /\
+    VerifyUnpackV3MatrixProfilePostFreeze.unpack_matrix_nonfirst_bound17
+      res.`2 /\
+    VerifyUnpackV3NttTightBoundPostFreeze.verify_unpack_ntt_input_signed131068
+      res.`1].
+proof.
+conseq
+  (actual_verify_unpack_post_decode_pre_ntt_mode2_word_exact
+     bp0 vkp0 mat0).
++ auto.
+move=> &m hpre result [hprefix [hframe hnonfirst]].
+have hsource :
+    VerifyUnpackV3PreNttBoundPostFreeze.pre_ntt_source_bound
+      vkp0 mat0 by
+  move: hpre => />.
+have hbound :=
+  VerifyUnpackV3PreNttTightBoundPostFreeze.pre_ntt_active_sint_bound_of_prefix_frame
+    vkp0 mat0 result.`2 result.`1 hsource hprefix hframe.
+have hinput :
+    VerifyUnpackV3NttTightBoundPostFreeze.verify_unpack_ntt_input_signed131068
+      result.`1.
++ move: hbound.
+  rewrite
+    /VerifyUnpackV3PreNttTightBoundPostFreeze.pre_ntt_active_sint_bound
+    /VerifyUnpackV3PreNttTightBoundPostFreeze.pre_ntt_sint_limit
+    /VerifyUnpackV3NttTightBoundPostFreeze.verify_unpack_ntt_input_signed131068
+    /VerifyUnpackV3NttTightBoundPostFreeze.signed_bound32
+    /VerifyUnpackV3NttTightBoundPostFreeze.verify_unpack_ntt_words
+    /VerifyUnpackV3NttTightBoundPostFreeze.verify_unpack_ntt_polys
+    /mode2_vec_words /mode2_rows /poly_words
+    /KeygenM23MatrixSpec.poly_words_i.
+  by auto.
+by auto.
+qed.
+
+lemma actual_verify_unpack_post_decode_pre_ntt_mode2_full_tight_input
+    (bp0 : BArray8192.t) (vkp0 : BArray2752.t)
+    (mat0 : BArray32768.t) :
+  hoare [ActualVerifyUnpackPostDecodePreNttMode2.run :
+    bp = bp0 /\ vkp = vkp0 /\ matp = mat0 /\
+    VerifyUnpackVkM23CoefficientsPostFreeze.decoded_coeff_prefix
+      bp0 vkp0 mode2_vec_words /\
+    VerifyUnpackV3ExpandBoundsPostFreeze.expanded_mode2_prefix_bound mat0 /\
+    VerifyUnpackV3PreNttBoundPostFreeze.pre_ntt_source_bound vkp0 mat0
+    ==>
+    VerifyUnpackV3PreNttPostFreeze.pre_ntt_prefix
+      vkp0 res.`2 res.`1 mode2_vec_words /\
+    mat_firstcol_frame mat0 res.`2 /\
+    VerifyUnpackV3MatrixProfilePostFreeze.unpack_matrix_nonfirst_bound17
+      res.`2 /\
+    VerifyUnpackV3NttBound17PostFreeze.verify_unpack_ntt_input_repr_bound17
+      res.`1
+      (KeygenM23ArithmeticSpec.wide_poly res.`1 0)
+      (KeygenM23ArithmeticSpec.wide_poly
+        res.`1 KeygenM23MatrixSpec.poly_words_i) /\
+    VerifyUnpackV3NttTightBoundPostFreeze.verify_unpack_ntt_input_signed131068
+      res.`1].
+proof.
+conseq
+  (actual_verify_unpack_post_decode_pre_ntt_mode2_bound17
+     bp0 vkp0 mat0)
+  (actual_verify_unpack_post_decode_pre_ntt_mode2_tight_bound
+     bp0 vkp0 mat0) => />.
+qed.
+
 module ActualVerifyUnpackPostDecodeThroughNttInstallMode2 = {
   proc run (bp : BArray8192.t, vkp : BArray2752.t,
             matp : BArray32768.t)
@@ -258,6 +337,99 @@ have hmatrixprofile :=
     (KeygenM23ArithmeticSpec.wide_poly
       pre_ntt0 KeygenM23MatrixSpec.poly_words_i)
     hnonfirst hnttbound hinstallprefix hmatrixframe.
+exists pre_ntt0 preinstall_mat0.
+by auto.
+qed.
+
+lemma actual_verify_unpack_post_decode_through_ntt_install_mode2_tight20_correct
+    (bp0 : BArray8192.t) (vkp0 : BArray2752.t)
+    (mat0 : BArray32768.t) :
+  hoare [ActualVerifyUnpackPostDecodeThroughNttInstallMode2.run :
+    bp = bp0 /\ vkp = vkp0 /\ matp = mat0 /\
+    VerifyUnpackVkM23CoefficientsPostFreeze.decoded_coeff_prefix
+      bp0 vkp0 mode2_vec_words /\
+    VerifyUnpackV3ExpandBoundsPostFreeze.expanded_mode2_prefix_bound mat0 /\
+    VerifyUnpackV3PreNttBoundPostFreeze.pre_ntt_source_bound vkp0 mat0
+    ==>
+    exists pre_ntt preinstall_mat,
+      VerifyUnpackV3PreNttPostFreeze.pre_ntt_prefix
+        vkp0 preinstall_mat pre_ntt mode2_vec_words /\
+      mat_firstcol_frame mat0 preinstall_mat /\
+      VerifyUnpackV3MatrixProfilePostFreeze.unpack_matrix_nonfirst_bound17
+        preinstall_mat /\
+      VerifyUnpackV3NttBound17PostFreeze.verify_unpack_ntt_input_repr_bound17
+        pre_ntt
+        (KeygenM23ArithmeticSpec.wide_poly pre_ntt 0)
+        (KeygenM23ArithmeticSpec.wide_poly
+          pre_ntt KeygenM23MatrixSpec.poly_words_i) /\
+      VerifyUnpackV3NttTightBoundPostFreeze.verify_unpack_ntt_input_signed131068
+        pre_ntt /\
+      VerifyUnpackV3NttTightBoundPostFreeze.verify_unpack_ntt_output_bound20
+        res.`1 /\
+      VerifyUnpackV3NttBound17PostFreeze.verify_unpack_ntt_repr_bound25
+        res.`1
+        (KeygenM23ArithmeticSpec.wide_poly pre_ntt 0)
+        (KeygenM23ArithmeticSpec.wide_poly
+          pre_ntt KeygenM23MatrixSpec.poly_words_i) /\
+      NTTRowProductSpec.vector_forward_repr
+        VerifyUnpackV3NttBound17PostFreeze.verify_unpack_ntt_polys
+        (fun col =>
+          KeygenM23ArithmeticSpec.wide_poly
+            res.`1 (col * KeygenM23MatrixSpec.poly_words_i))
+        (fun col =>
+          KeygenM23ArithmeticSpec.wide_poly
+            pre_ntt (col * KeygenM23MatrixSpec.poly_words_i)) /\
+      KeygenM23MatrixSpec.word_tail_frame
+        pre_ntt res.`1
+          VerifyUnpackV3NttBound17PostFreeze.verify_unpack_ntt_words /\
+      mat_firstcol_install_prefix res.`1 res.`2 mode2_vec_words /\
+      mat_firstcol_install_frame
+        preinstall_mat res.`2 mode2_vec_words /\
+      VerifyUnpackV3MatrixProfilePostFreeze.verify_unpack_mode2_matrix_repr_bound20_17
+        res.`2].
+proof.
+proc.
+seq 1 :
+  (exists pre_ntt preinstall_mat,
+     bp = pre_ntt /\ vkp = vkp0 /\ matp = preinstall_mat /\
+     VerifyUnpackV3PreNttPostFreeze.pre_ntt_prefix
+       vkp0 preinstall_mat pre_ntt mode2_vec_words /\
+     mat_firstcol_frame mat0 preinstall_mat /\
+     VerifyUnpackV3MatrixProfilePostFreeze.unpack_matrix_nonfirst_bound17
+       preinstall_mat /\
+     VerifyUnpackV3NttBound17PostFreeze.verify_unpack_ntt_input_repr_bound17
+       pre_ntt
+       (KeygenM23ArithmeticSpec.wide_poly pre_ntt 0)
+       (KeygenM23ArithmeticSpec.wide_poly
+         pre_ntt KeygenM23MatrixSpec.poly_words_i) /\
+     VerifyUnpackV3NttTightBoundPostFreeze.verify_unpack_ntt_input_signed131068
+       pre_ntt).
++ call
+    (actual_verify_unpack_post_decode_pre_ntt_mode2_full_tight_input
+       bp0 vkp0 mat0).
+  auto => />.
+  move=> result hprefix hframe hnonfirst hinput0 hinput1 hsigned.
+  smt().
+exlim bp => pre_ntt0.
+exlim matp => preinstall_mat0.
+call
+  (VerifyUnpackV3NttInstallPostFreeze.actual_verify_unpack_ntt_install_mode2_full_correct_tight20
+     pre_ntt0 preinstall_mat0
+     (KeygenM23ArithmeticSpec.wide_poly pre_ntt0 0)
+     (KeygenM23ArithmeticSpec.wide_poly
+       pre_ntt0 KeygenM23MatrixSpec.poly_words_i)).
+auto => />.
+move=> &m hprefix hmatframe hnonfirst hinput0 hinput1 hsigned
+        result htight hntt0 hntt0bound hntt1 hntt1bound
+        hforward htail hinstall hinstallframe.
+have hnttbound :
+    VerifyUnpackV3NttTightBoundPostFreeze.verify_unpack_ntt_output_bound20
+      result.`1 by
+  exact htight.
+have hmatrixprofile :=
+  VerifyUnpackV3MatrixProfilePostFreeze.verify_unpack_mode2_matrix_repr_bound20_17_of_install
+    result.`1 preinstall_mat0 result.`2
+    hnonfirst hnttbound hinstall hinstallframe.
 exists pre_ntt0 preinstall_mat0.
 by auto.
 qed.
